add td interface locale chain

src/Solver/TD_Interface.thy
@@ -1,386 +1,64 @@
 theory TD_Interface
-  imports Constraint_System CFG_Runs_To_Bridge "TD.TD_plain"
+  imports TD_CFG_Core "TD.TD_plain"
 begin
 
-(*
-  Top-Down Solver Interface.
-
-  We connect our function-style RHS
-    rhs :: pp => (pp => 'a abs_state) => 'a abs_state
-  to AFP's strategy-tree interface
-    T   :: pp => (pp, 'a abs_state) strategy_tree.
-*)
-
-(* -- Monotone RHS wrapper (reused in downstream proofs) -- *)
-
-definition make_rhs ::
-    "cfg
-     => 'a::ord domain_transfer
-     => ('a abs_state => 'a abs_state => 'a abs_state)
-     => 'a abs_state
-     => 'a abs_state
-     => pp => (pp => 'a abs_state) => 'a abs_state"
-where
-  "make_rhs g tf join_abs bot_abs s0 v env =
-     rhs g tf join_abs bot_abs s0 env v"
-
-lemma make_rhs_mono:
-  assumes fin: "finite (edges g)"
-  assumes cfu: "comp_fun_commute (join_abs :: 'a::preorder abs_state \<Rightarrow> 'a abs_state \<Rightarrow> 'a abs_state)"
-  assumes join_ub1: "\<And>x y::'a abs_state. x \<le> join_abs x y"
-  assumes join_ub2: "\<And>x y::'a abs_state. y \<le> join_abs x y"
-  assumes join_mono:
-      "\<And>x1 y1 x2 y2::'a abs_state. x1 \<le> y1 \<Longrightarrow> x2 \<le> y2 \<Longrightarrow> join_abs x1 x2 \<le> join_abs y1 y2"
-  assumes join_least:
-      "\<And>x y z::'a abs_state. x \<le> z \<Longrightarrow> y \<le> z \<Longrightarrow> join_abs x y \<le> z"
-  assumes tf_mono:
-      "\<And>a \<sigma>1 \<sigma>2::'a abs_state. \<sigma>1 \<le> \<sigma>2 \<Longrightarrow> apply_tf tf a \<sigma>1 \<le> apply_tf tf a \<sigma>2"
-  shows "monotone (\<le>) (\<le>) (make_rhs g tf join_abs bot_abs s0 v)"
-proof (rule monotoneI)
-  fix env1 env2 :: "pp \<Rightarrow> 'a abs_state"
-  assume "env1 \<le> env2"
-  then have env_le: "\<forall>v. env1 v \<le> env2 v"
-    by (simp add: le_fun_def)
-  show "make_rhs g tf join_abs bot_abs s0 v env1 \<le> make_rhs g tf join_abs bot_abs s0 v env2"
-    unfolding make_rhs_def
-    by (rule rhs_mono[OF fin cfu join_ub1 join_ub2 join_mono join_least tf_mono env_le])
-qed
-
-(* -- Strategy-tree bridge to AFP TD_plain -- *)
-
-fun rhs_tree_fold ::
-    "'a domain_transfer
-     => ('a abs_state => 'a abs_state => 'a abs_state)
-     => 'a abs_state
-     => (pp * edge_action) list
-     => (pp, 'a abs_state) strategy_tree"
-where
-  "rhs_tree_fold tf join_abs acc [] = Answer acc"
-| "rhs_tree_fold tf join_abs acc ((u,a)#ps) =
-     Query u (\<lambda>su. rhs_tree_fold tf join_abs (join_abs acc (apply_tf tf a su)) ps)"
-
-definition make_rhs_tree ::
-    "cfg
-     => 'a domain_transfer
-     => ('a abs_state => 'a abs_state => 'a abs_state)
-     => 'a abs_state
-     => 'a abs_state
-     => pp
-     => (pp, 'a abs_state) strategy_tree"
-where
-  "make_rhs_tree g tf join_abs bot_abs s0 v =
-     (let acc0 = (if v = cfg_entry g then join_abs bot_abs s0 else bot_abs)
-      in rhs_tree_fold tf join_abs acc0 (predecessor_list g v))"
-
-definition env_map :: "(pp => 'a abs_state) => (pp, 'a abs_state) map" where
-  "env_map env = (\<lambda>x. Some (env x))"
-
-definition lookup_bot :: "('x, 'd::bot) map => 'x => 'd" where
-  "lookup_bot m x = (case m x of None => bot | Some d => d)"
-
-lemma lookup_bot_env_map[simp]:
-  "lookup_bot (env_map env) x = env x"
-  unfolding lookup_bot_def env_map_def
-  by simp
-
-lemma mlup_env_map[simp]:
-  fixes env :: "pp \<Rightarrow> ('a::{bot}) abs_state"
-  shows "mlup (env_map env) x = env x"
-  unfolding mlup_def env_map_def by simp
-
-lemma rhs_tree_fold_traverse_env_map:
-  fixes env :: "pp \<Rightarrow> ('a::bounded_semilattice_sup_bot) abs_state"
-  shows "traverse_rhs (rhs_tree_fold tf join_abs acc ps) (env_map env)
-     = fold (\<lambda>(u,a) st. join_abs st (apply_tf tf a (env u))) ps acc"
-proof (induct ps arbitrary: acc)
-  case Nil
-  show ?case
-    by simp
-next
-  case (Cons p ps)
-  obtain u a where p: "p = (u, a)"
-    by (cases p) auto
-  have "traverse_rhs (rhs_tree_fold tf join_abs acc (p # ps)) (env_map env) =
-        traverse_rhs (Query u (\<lambda>su. rhs_tree_fold tf join_abs (join_abs acc (apply_tf tf a su)) ps))
-         (env_map env)"
-    by (simp add: p)
-  also have "\<dots> =
-        traverse_rhs (rhs_tree_fold tf join_abs (join_abs acc (apply_tf tf a (env u))) ps)
-         (env_map env)"
-    by simp
-  also have "\<dots> =
-        fold (\<lambda>(u,a) st. join_abs st (apply_tf tf a (env u))) ps
-         (join_abs acc (apply_tf tf a (env u)))"
-    using Cons[of "join_abs acc (apply_tf tf a (env u))"] by simp
-  also have "\<dots> =
-        fold (\<lambda>(u,a) st. join_abs st (apply_tf tf a (env u))) (p # ps) acc"
-    by (simp add: p)
-  finally show ?case .
-qed
-
-(* Avoid simp turning @{text "set xs = {}"} inside @{text SOME} into @{text "xs = []"} the wrong way. *)
-lemma SOME_list_distinct_set_empty_eq_Nil:
-  "(SOME xs :: ('a::type) list. distinct xs \<and> set xs = {}) = []"
-proof (rule some_equality)
-  show "distinct ([] :: 'a list) \<and> set [] = {}"
-    by simp
-next
-  fix xs :: "'a list"
-  assume H: "distinct xs \<and> set xs = {}"
-  then show "xs = []"
-    by simp
-qed
-
-lemma SOME_distinct_list_if_set_empty:
-  fixes P :: "'a set"
-  assumes hp: "P = {}"
-  shows "(SOME xs :: 'a list. distinct xs \<and> set xs = P) = []"
-  unfolding hp by (rule SOME_list_distinct_set_empty_eq_Nil)
-
-(* Special case: no edges into v and v is not the entry tree is Answer bot, same as rhs. *)
-lemma make_rhs_tree_eq_Answer_bot_if_no_preds_not_entry:
-  assumes not_e: "v \<noteq> cfg_entry g"
-  assumes no_in: "\<And>u a. (u, a, v) \<notin> edges g"
-  shows "make_rhs_tree g tf join_abs bot_abs s0 v = Answer bot_abs"
-  unfolding make_rhs_tree_def Let_def
-  using no_in not_e predecessor_list_Nil_if_no_in
-  by simp
-
-lemma make_rhs_tree_correspondence_not_entry_no_predecessors:
-  fixes env :: "pp \<Rightarrow> ('a::bounded_semilattice_sup_bot) abs_state"
-  assumes not_e: "v \<noteq> cfg_entry g"
-  assumes no_in: "\<And>u a. (u, a, v) \<notin> edges g"
-  shows "traverse_rhs (make_rhs_tree g tf join_abs bot_abs s0 v) (env_map env) =
-         make_rhs g tf join_abs bot_abs s0 v env"
-proof -
-  have tr: "traverse_rhs (make_rhs_tree g tf join_abs bot_abs s0 v) (env_map env) = bot_abs"
-    unfolding make_rhs_tree_eq_Answer_bot_if_no_preds_not_entry[OF not_e no_in] by simp
-  have mk: "make_rhs g tf join_abs bot_abs s0 v env = bot_abs"
-    unfolding make_rhs_def by (simp add: rhs_no_predecessors_not_entry not_e no_in)
-  from tr mk show ?thesis
-    by simp
-qed
-
-lemma finite_predecessor_pairs:
-  assumes fin: "finite (edges g)"
-  shows "finite {(u,a). (u,a,v) \<in> edges g}"
-proof (rule finite_subset)
-  show "{(u,a). (u,a,v) \<in> edges g} \<subseteq> (\<lambda>(u, a, w). (u, a)) ` edges g"
-    by force
-  show "finite ((\<lambda>(u, a, w). (u, a)) ` edges g)"
-    by (simp add: fin)
-qed
-
-lemma fold_join_apply_edges_eq_fold_join_over_map:
-  fixes join :: "'a \<Rightarrow> 'a \<Rightarrow> 'a" and F :: "('b \<times> 'c) \<Rightarrow> 'a"
-  shows "fold (\<lambda>p acc. join (F p) acc) ps acc =
-         fold (\<lambda>x acc. join x acc) (map F ps) acc"
-proof (induct ps arbitrary: acc)
-  case Nil
-  show ?case
-    by simp
-next
-  case (Cons p ps)
-  have "fold (\<lambda>p acc. join (F p) acc) (p # ps) acc =
-        fold (\<lambda>p acc. join (F p) acc) ps (join (F p) acc)"
-    by simp
-  also have "\<dots> = fold (\<lambda>x acc. join x acc) (map F ps) (join (F p) acc)"
-    using Cons[of "join (F p) acc"] by simp
-  also have "\<dots> = fold (\<lambda>x acc. join x acc) (map F (p # ps)) acc"
-    by simp
-  finally show ?case .
-qed
-
-lemma rhs_eq_fold_predecessors:
-  fixes g v tf join_abs bot_abs s0
-  fixes env :: "pp \<Rightarrow> ('a::bounded_semilattice_sup_bot) abs_state"
-  assumes fin: "finite (edges g)"
-  assumes cfi: "comp_fun_idem (join_abs :: 'a abs_state \<Rightarrow> 'a abs_state \<Rightarrow> 'a abs_state)"
-  assumes join_sym: "\<And>x y. join_abs x y = join_abs y x"
-  assumes dist: "distinct ps"
-  assumes setps: "set ps = {(u,a). (u,a,v) \<in> edges g}"
-  defines "preds \<equiv> {(u,a). (u,a,v) \<in> edges g}"
-  defines "F \<equiv> (\<lambda>(u,a). apply_tf tf a (env u))"
-  defines "vals \<equiv> F ` preds"
-  defines "acc0 \<equiv> (if v = cfg_entry g then join_abs bot_abs s0 else bot_abs)"
-  shows "rhs g tf join_abs bot_abs s0 env v =
-         fold (\<lambda>(u,a) acc. join_abs (apply_tf tf a (env u)) acc) ps acc0"
-proof -
-  interpret j: comp_fun_idem join_abs
-    by (fact cfi)
-  have fin_preds: "finite preds"
-    unfolding preds_def by (rule finite_predecessor_pairs[OF fin])
-  have setps': "set ps = preds"
-    unfolding preds_def using setps by simp
-  have vals_eq: "vals = set (map F ps)"
-    unfolding vals_def using setps' by simp
-  have fold_map:
-    "fold (\<lambda>(u,a) acc. join_abs (apply_tf tf a (env u)) acc) ps acc0 =
-     fold (\<lambda>x acc. join_abs x acc) (map F ps) acc0"
-  proof -
-    have H: "(\<lambda>(u,a) acc. join_abs (apply_tf tf a (env u)) acc) = (\<lambda>p acc. join_abs (F p) acc)"
-      by (rule ext)+ (simp add: F_def split: prod.split)
-    show ?thesis
-      unfolding H by (rule fold_join_apply_edges_eq_fold_join_over_map)
-  qed
-  have fold_set:
-    "Finite_Set.fold join_abs acc0 (set (map F ps)) =
-     fold (\<lambda>x acc. join_abs x acc) (map F ps) acc0"
-    by (rule j.fold_set_fold)
-  show ?thesis
-  proof (cases "v = cfg_entry g")
-    case True
-    have rhsv: "rhs g tf join_abs bot_abs s0 env v = abs_join_set join_abs bot_abs (insert s0 vals)"
-      unfolding rhs_def preds_def vals_def F_def using True by (simp add: Let_def)
-    have fin_vals: "finite vals"
-      unfolding vals_def using fin_preds by simp
-    have ins_fold:
-      "Finite_Set.fold join_abs bot_abs (insert s0 vals) =
-       Finite_Set.fold join_abs (join_abs s0 bot_abs) vals"
-      by (simp only: j.fold_insert_idem2 fin_vals)
-    also have "join_abs s0 bot_abs = join_abs bot_abs s0"
-      by (simp add: join_sym)
-    also have "Finite_Set.fold join_abs (join_abs bot_abs s0) vals =
-               Finite_Set.fold join_abs acc0 (set (map F ps))"
-      unfolding vals_eq acc0_def using True by simp
-    also have "\<dots> = fold (\<lambda>x acc. join_abs x acc) (map F ps) acc0"
-      by (simp add: fold_set[symmetric])
-    also have "\<dots> = fold (\<lambda>(u,a) acc. join_abs (apply_tf tf a (env u)) acc) ps acc0"
-      by (simp add: fold_map[symmetric])
-    finally show ?thesis
-      unfolding rhsv abs_join_set_def by simp
-  next
-    case False
-    then have ne: "v \<noteq> cfg_entry g"
-      by simp
-    have rhsv: "rhs g tf join_abs bot_abs s0 env v = abs_join_set join_abs bot_abs vals"
-      unfolding rhs_def preds_def vals_def F_def using False by (simp add: Let_def)
-    have "Finite_Set.fold join_abs bot_abs vals =
-          Finite_Set.fold join_abs acc0 (set (map F ps))"
-      unfolding vals_eq acc0_def using ne by simp
-    also have "\<dots> = fold (\<lambda>x acc. join_abs x acc) (map F ps) acc0"
-      by (simp add: fold_set[symmetric])
-    also have "\<dots> = fold (\<lambda>(u,a) acc. join_abs (apply_tf tf a (env u)) acc) ps acc0"
-      by (simp add: fold_map[symmetric])
-    finally show ?thesis
-      unfolding rhsv abs_join_set_def by simp
-  qed
-qed
-
-lemma rhs_eq_fold_predecessor_list:
-  fixes g v tf join_abs bot_abs s0
-  fixes env :: "pp \<Rightarrow> ('a::bounded_semilattice_sup_bot) abs_state"
-  assumes fin: "finite (edges g)"
-  assumes cfi: "comp_fun_idem (join_abs :: 'a abs_state \<Rightarrow> 'a abs_state \<Rightarrow> 'a abs_state)"
-  assumes join_sym: "\<And>x y. join_abs x y = join_abs y x"
-  shows "rhs g tf join_abs bot_abs s0 env v =
-         fold (\<lambda>(u,a) acc. join_abs (apply_tf tf a (env u)) acc)
-              (predecessor_list g v)
-              (if v = cfg_entry g then join_abs bot_abs s0 else bot_abs)"
-proof -
-  have setps: "set (predecessor_list g v) = {(u,a). (u,a,v) \<in> edges g}"
-    using set_predecessor_list[OF fin] unfolding predecessors_def by auto
-  show ?thesis
-    using rhs_eq_fold_predecessors[OF fin cfi join_sym
-        distinct_predecessor_list[OF fin] setps]
-    by simp
-qed
-
-lemma fold_join_abs_swap_edge_steps:
-  fixes join_abs :: "'a::bounded_semilattice_sup_bot abs_state \<Rightarrow> 'a abs_state \<Rightarrow> 'a abs_state"
-    and tf :: "'a domain_transfer"
-    and env :: "pp \<Rightarrow> 'a abs_state"
-  assumes join_sym: "\<And>x y. join_abs x y = join_abs y x"
-  shows "fold (\<lambda>(u,a) st. join_abs st (apply_tf tf a (env u))) ps acc =
-         fold (\<lambda>(u,a) acc. join_abs (apply_tf tf a (env u)) acc) ps acc"
-proof (induct ps arbitrary: acc)
-  case Nil
-  show ?case
-    by simp
-next
-  case (Cons p ps)
-  obtain u a where pa: "p = (u, a)"
-    by (cases p) auto
-  have "fold (\<lambda>(u,a) st. join_abs st (apply_tf tf a (env u))) (p # ps) acc =
-        fold (\<lambda>(u,a) st. join_abs st (apply_tf tf a (env u))) ps (join_abs acc (apply_tf tf a (env u)))"
-    by (simp add: pa)
-  also have "join_abs acc (apply_tf tf a (env u)) = join_abs (apply_tf tf a (env u)) acc"
-    by (simp add: join_sym)
-  also have "fold (\<lambda>(u,a) st. join_abs st (apply_tf tf a (env u))) ps (join_abs (apply_tf tf a (env u)) acc) =
-             fold (\<lambda>(u,a) acc. join_abs (apply_tf tf a (env u)) acc) ps (join_abs (apply_tf tf a (env u)) acc)"
-    using Cons.hyps by simp
-  also have "\<dots> = fold (\<lambda>(u,a) acc. join_abs (apply_tf tf a (env u)) acc) (p # ps) acc"
-    by (simp add: pa)
-  finally show ?case .
-qed
-
-lemma make_rhs_tree_correspondence:
-  assumes fin: "finite (edges g)"
-  assumes cfi: "comp_fun_idem (join_abs :: 'a::bounded_semilattice_sup_bot abs_state \<Rightarrow> 'a abs_state \<Rightarrow> 'a abs_state)"
-  assumes join_sym: "\<And>x y. join_abs x y = join_abs y x"
-  shows "traverse_rhs (make_rhs_tree g tf join_abs bot_abs s0 v) (env_map (env :: pp \<Rightarrow> 'a abs_state)) =
-         make_rhs g tf join_abs bot_abs s0 v env"
-proof -
-  have "traverse_rhs (make_rhs_tree g tf join_abs bot_abs s0 v) (env_map env) =
-        fold (\<lambda>(u,a) st. join_abs st (apply_tf tf a (env u)))
-             (predecessor_list g v)
-             (if v = cfg_entry g then join_abs bot_abs s0 else bot_abs)"
-    unfolding make_rhs_tree_def Let_def
-    by (simp add: rhs_tree_fold_traverse_env_map)
-  also have "\<dots> =
-        fold (\<lambda>(u,a) acc. join_abs (apply_tf tf a (env u)) acc)
-             (predecessor_list g v)
-             (if v = cfg_entry g then join_abs bot_abs s0 else bot_abs)"
-    by (rule fold_join_abs_swap_edge_steps[OF join_sym])
-  also have "\<dots> = rhs g tf join_abs bot_abs s0 env v"
-    by (simp add: rhs_eq_fold_predecessor_list[OF fin cfi join_sym])
-  finally show ?thesis
-    unfolding make_rhs_def by (simp split: if_splits)
-qed
-
-lemma mlup_env_map_of_mlup:
-  fixes \<sigma> :: "(pp, ('a::bounded_semilattice_sup_bot) abs_state) map"
-  shows "mlup (env_map (\<lambda>w. mlup \<sigma> w)) x = mlup \<sigma> x"
-  by (simp add: mlup_env_map)
-
-lemma lookup_bot_mlup:
-  fixes \<sigma> :: "(pp, ('a::bounded_semilattice_sup_bot) abs_state) map"
-  shows "lookup_bot \<sigma> x = mlup \<sigma> x"
-  unfolding lookup_bot_def mlup_def by (cases "\<sigma> x") simp_all
-
-lemma traverse_rhs_mlup_eq:
-  fixes t :: "(pp, ('a::bounded_semilattice_sup_bot) abs_state) strategy_tree"
-    and \<sigma> \<sigma>' :: "(pp, ('a::bounded_semilattice_sup_bot) abs_state) map"
-  assumes mlup_ag: "\<And>z. mlup \<sigma> z = mlup \<sigma>' z"
-  shows "traverse_rhs t \<sigma> = traverse_rhs t \<sigma>'"
-  apply (rule solution_sufficient_t)
-  using mlup_ag by simp
-
-lemma rhs_make_rhs_tree_traverse_mlup:
-  fixes g :: cfg and tf :: "'a::bounded_semilattice_sup_bot domain_transfer"
-    and join_abs bot_abs s0 v and \<sigma> :: "(pp, ('a::bounded_semilattice_sup_bot) abs_state) map"
-  assumes fin: "finite (edges g)"
-  assumes cfi: "comp_fun_idem (join_abs :: 'a abs_state \<Rightarrow> 'a abs_state \<Rightarrow> 'a abs_state)"
-  assumes join_sym: "\<And>x y. join_abs x y = join_abs y x"
-  shows "rhs g tf join_abs bot_abs s0 (\<lambda>w. mlup \<sigma> w) v =
-         traverse_rhs (make_rhs_tree g tf join_abs bot_abs s0 v) \<sigma>"
-proof -
-  have "traverse_rhs (make_rhs_tree g tf join_abs bot_abs s0 v) \<sigma> =
-        traverse_rhs (make_rhs_tree g tf join_abs bot_abs s0 v) (env_map (\<lambda>w. mlup \<sigma> w))"
-    by (rule traverse_rhs_mlup_eq) (simp add: mlup_env_map_of_mlup)
-  also have "\<dots> =
-        make_rhs g tf join_abs bot_abs s0 v (\<lambda>w. mlup \<sigma> w)"
-    by (simp add: make_rhs_tree_correspondence[OF fin cfi join_sym])
-  also have "\<dots> = rhs g tf join_abs bot_abs s0 (\<lambda>w. mlup \<sigma> w) v"
-    by (simp add: make_rhs_def)
-  finally show ?thesis ..
-qed
+(* Plain TD backend (join only, no widening). *)
 
 lemma part_solutionD:
   fixes T v0 sigma v
   assumes "part_solution T v0 sigma (reach T sigma v0)" and "v \<in> reach T sigma v0"
   shows "eq T v sigma = mlup sigma v"
   using assms by auto
+
+locale td_cfg_plain_solver = td_cfg_core + TD_plain cfg_T
+begin
+
+definition td_sigma :: "(pp, 'a abs_state) map"
+where
+  "td_sigma = TD_plain_Interp_solve cfg_T (cfg_entry g)"
+
+definition td_env :: "pp \<Rightarrow> 'a abs_state"
+where
+  "td_env v = lookup_bot td_sigma v"
+
+lemma td_sigma_solve:
+  "TD_plain_Interp_solve cfg_T (cfg_entry g) = td_sigma"
+  unfolding td_sigma_def by simp
+
+lemma td_plain_part_solution:
+  assumes dom: "TD_plain.solve_dom cfg_T (cfg_entry g)"
+  shows "part_solution cfg_T (cfg_entry g) td_sigma (reach cfg_T td_sigma (cfg_entry g))"
+proof (rule TD_plain_Interp.partial_correctness)
+  show "TD_plain.solve_dom cfg_T (cfg_entry g)"
+    by (fact dom)
+  show "TD_plain_Interp_solve cfg_T (cfg_entry g) = td_sigma"
+    by (simp add: td_sigma_solve)
+qed
+
+lemma td_env_post_fixpoint:
+  assumes fin: "finite (edges g)"
+  assumes cfi: "comp_fun_idem join_abs"
+  assumes join_sym: "\<And>x y. join_abs x y = join_abs y x"
+  assumes dom: "TD_plain.solve_dom cfg_T (cfg_entry g)"
+  assumes reach: "\<And>v. v \<in> reach cfg_T td_sigma (cfg_entry g)"
+  shows "is_post_fixpoint g tf join_abs bot_abs s0 td_env"
+proof (rule cfg_env_post_fixpoint[where env=td_env and \<sigma>=td_sigma, OF fin cfi join_sym])
+  show "\<And>w. td_env w = lookup_bot td_sigma w"
+    unfolding td_env_def by simp
+next
+  fix v
+  show "(eq cfg_T) v td_sigma \<le> mlup td_sigma v"
+  proof -
+    have v_reach: "v \<in> reach cfg_T td_sigma (cfg_entry g)"
+      using reach by simp
+    have psol: "part_solution cfg_T (cfg_entry g) td_sigma (reach cfg_T td_sigma (cfg_entry g))"
+      using td_plain_part_solution[OF dom] .
+    show ?thesis
+      using part_solutionD[OF psol v_reach] by simp
+  qed
+qed
+
+end
 
 definition td_analyse ::
     "com
@@ -390,23 +68,16 @@ definition td_analyse ::
      => 'a abs_state
      => pp => 'a abs_state"
 where
-  "td_analyse c tf join_abs bot_abs s0 =
-     (let g = to_cfg c;
-          T = make_rhs_tree g tf join_abs bot_abs s0;
-          \<sigma> = TD_plain_Interp_solve T (cfg_entry g)
-      in (\<lambda>v. lookup_bot \<sigma> v))"
+  "td_analyse c tf join_abs bot_abs s0 v =
+     lookup_bot (TD_plain_Interp_solve (make_rhs_tree (to_cfg c) tf join_abs bot_abs s0)
+                   (cfg_entry (to_cfg c))) v"
 
-(*
-  Post-fixpoint of td_analyse (TD solver output read back as an environment):
+lemma td_analyse_def_expand:
+  "td_analyse c tf join_abs bot_abs s0 v =
+     lookup_bot (TD_plain_Interp_solve (make_rhs_tree (to_cfg c) tf join_abs bot_abs s0)
+                   (cfg_entry (to_cfg c))) v"
+  unfolding td_analyse_def by simp
 
-  Uses AFP TD_plain.partial_correctness (part_solution on the reach set from the
-  queried CFG entry) plus make_rhs_tree_correspondence.
-
-  Extra assumptions beyond finiteness / join algebra:
-    - TD_plain.solve_dom for the strategy forest rooted at cfg_entry
-    - every program point lies in the solver reach set from that entry
-      (typically discharged from CFG shape / compile for whole-program analysis).
-*)
 theorem td_analyse_post_fixpoint:
   fixes c tf join_abs bot_abs s0
   assumes fin: "finite (edges (to_cfg c))"
@@ -421,46 +92,25 @@ theorem td_analyse_post_fixpoint:
                     (cfg_entry (to_cfg c))"
   shows "is_post_fixpoint (to_cfg c) tf join_abs bot_abs s0
            (td_analyse c tf join_abs bot_abs s0)"
-proof (unfold is_post_fixpoint_def td_analyse_def, intro allI)
-  fix v
-  define g where "g = to_cfg c"
-  define T where "T = make_rhs_tree g tf join_abs bot_abs s0"
-  define v0 where "v0 = cfg_entry g"
-  define \<sigma> where "\<sigma> = TD_plain_Interp_solve T v0"
-  have fin_g: "finite (edges g)"
-    unfolding g_def using fin by simp
-  have psol: "part_solution T v0 \<sigma> (reach T \<sigma> v0)"
-  proof (rule TD_plain_Interp.partial_correctness)
-    show "TD_plain.solve_dom T v0"
-      unfolding T_def v0_def g_def by (fact solve_dom)
-  next
-    show "TD_plain_Interp_solve T v0 = \<sigma>"
-      by (simp add: \<sigma>_def)
+proof -
+  interpret plain: td_cfg_plain_solver "to_cfg c" tf join_abs bot_abs s0 .
+  have dom': "TD_plain.solve_dom plain.cfg_T (cfg_entry (to_cfg c))"
+  proof -
+    have "plain.cfg_T = make_rhs_tree (to_cfg c) tf join_abs bot_abs s0"
+      by (simp add: fun_eq_iff plain.cfg_T_eq)
+    then show ?thesis using solve_dom by simp
   qed
-  have v_reach: "v \<in> reach T \<sigma> v0"
-    unfolding g_def T_def v0_def \<sigma>_def using cfg_in_reach by simp
-  have eqv: "eq T v \<sigma> = mlup \<sigma> v"
-    by (rule part_solutionD[OF psol v_reach])
-  have env_mlup: "(\<lambda>w. mlup \<sigma> w) = (\<lambda>w. lookup_bot \<sigma> w)"
-    by (simp add: fun_eq_iff lookup_bot_mlup)
-  have "rhs g tf join_abs bot_abs s0 (\<lambda>w. lookup_bot \<sigma> w) v =
-        rhs g tf join_abs bot_abs s0 (\<lambda>w. mlup \<sigma> w) v"
-    by (simp add: env_mlup)
-  also have "\<dots> = traverse_rhs (T v) \<sigma>"
-    unfolding T_def by (simp add: rhs_make_rhs_tree_traverse_mlup[OF fin_g cfi join_sym])
-  also have "\<dots> = eq T v \<sigma>"
-    by (simp only: eq_def[symmetric])
-  also have "\<dots> = mlup \<sigma> v"
-    by (simp only: eqv)
-  also have "\<dots> = lookup_bot \<sigma> v"
-    by (simp add: lookup_bot_mlup)
-  finally have rhs_lookup: "rhs g tf join_abs bot_abs s0 (\<lambda>w. lookup_bot \<sigma> w) v = lookup_bot \<sigma> v" .
-  show "rhs (to_cfg c) tf join_abs bot_abs s0
-          (let g = to_cfg c; T = make_rhs_tree g tf join_abs bot_abs s0
-           in Let (TD_plain_Interp_solve T (cfg_entry g)) lookup_bot) v
-        \<le> (let g = to_cfg c; T = make_rhs_tree g tf join_abs bot_abs s0
-            in Let (TD_plain_Interp_solve T (cfg_entry g)) lookup_bot) v"
-    by (simp add: Let_def g_def[symmetric] T_def[symmetric] v0_def[symmetric] \<sigma>_def[symmetric] rhs_lookup)
+  have cfg_T: "plain.cfg_T = make_rhs_tree (to_cfg c) tf join_abs bot_abs s0"
+    by (simp add: fun_eq_iff plain.cfg_T_eq)
+  have env_eq: "td_analyse c tf join_abs bot_abs s0 = plain.td_env"
+    unfolding td_analyse_def plain.td_env_def plain.td_sigma_def
+    using cfg_T
+    by (intro ext, simp)  have reach': "\<And>v. v \<in> reach plain.cfg_T plain.td_sigma (cfg_entry (to_cfg c))"
+    using cfg_in_reach
+    by (simp add: plain.td_sigma_def cfg_T fun_eq_iff)
+  show ?thesis
+    unfolding env_eq
+    using plain.td_env_post_fixpoint[OF fin cfi join_sym dom' reach'] .
 qed
 
 end
