src/Solver/TD_CFG_Core.thy
@@ -1,0 +1,464 @@
+theory TD_CFG_Core
+  imports Constraint_System CFG_Runs_To_Bridge "TD.Basics"
+begin
+
+(*
+  Top-Down Solver Interface.
+
+  We connect our function-style RHS
+    rhs :: pp => (pp => 'a abs_state) => 'a abs_state
+  to AFP's strategy-tree interface
+    T   :: pp => (pp, 'a abs_state) strategy_tree.
+*)
+
+(* -- Monotone RHS wrapper (reused in downstream proofs) -- *)
+
+definition make_rhs ::
+    "cfg
+     => 'a::ord domain_transfer
+     => ('a abs_state => 'a abs_state => 'a abs_state)
+     => 'a abs_state
+     => 'a abs_state
+     => pp => (pp => 'a abs_state) => 'a abs_state"
+where
+  "make_rhs g tf join_abs bot_abs s0 v env =
+     rhs g tf join_abs bot_abs s0 env v"
+
+lemma make_rhs_mono:
+  assumes fin: "finite (edges g)"
+  assumes cfu: "comp_fun_commute (join_abs :: 'a::preorder abs_state \<Rightarrow> 'a abs_state \<Rightarrow> 'a abs_state)"
+  assumes join_ub1: "\<And>x y::'a abs_state. x \<le> join_abs x y"
+  assumes join_ub2: "\<And>x y::'a abs_state. y \<le> join_abs x y"
+  assumes join_mono:
+      "\<And>x1 y1 x2 y2::'a abs_state. x1 \<le> y1 \<Longrightarrow> x2 \<le> y2 \<Longrightarrow> join_abs x1 x2 \<le> join_abs y1 y2"
+  assumes join_least:
+      "\<And>x y z::'a abs_state. x \<le> z \<Longrightarrow> y \<le> z \<Longrightarrow> join_abs x y \<le> z"
+  assumes tf_mono:
+      "\<And>a \<sigma>1 \<sigma>2::'a abs_state. \<sigma>1 \<le> \<sigma>2 \<Longrightarrow> apply_tf tf a \<sigma>1 \<le> apply_tf tf a \<sigma>2"
+  shows "monotone (\<le>) (\<le>) (make_rhs g tf join_abs bot_abs s0 v)"
+proof (rule monotoneI)
+  fix env1 env2 :: "pp \<Rightarrow> 'a abs_state"
+  assume "env1 \<le> env2"
+  then have env_le: "\<forall>v. env1 v \<le> env2 v"
+    by (simp add: le_fun_def)
+  show "make_rhs g tf join_abs bot_abs s0 v env1 \<le> make_rhs g tf join_abs bot_abs s0 v env2"
+    unfolding make_rhs_def
+    by (rule rhs_mono[OF fin cfu join_ub1 join_ub2 join_mono join_least tf_mono env_le])
+qed
+
+(* -- Strategy-tree bridge to AFP TD_plain -- *)
+
+fun rhs_tree_fold ::
+    "'a domain_transfer
+     => ('a abs_state => 'a abs_state => 'a abs_state)
+     => 'a abs_state
+     => (pp * edge_action) list
+     => (pp, 'a abs_state) strategy_tree"
+where
+  "rhs_tree_fold tf join_abs acc [] = Answer acc"
+| "rhs_tree_fold tf join_abs acc ((u,a)#ps) =
+     Query u (\<lambda>su. rhs_tree_fold tf join_abs (join_abs acc (apply_tf tf a su)) ps)"
+
+definition make_rhs_tree ::
+    "cfg
+     => 'a domain_transfer
+     => ('a abs_state => 'a abs_state => 'a abs_state)
+     => 'a abs_state
+     => 'a abs_state
+     => pp
+     => (pp, 'a abs_state) strategy_tree"
+where
+  "make_rhs_tree g tf join_abs bot_abs s0 v =
+     (let acc0 = (if v = cfg_entry g then join_abs bot_abs s0 else bot_abs)
+      in rhs_tree_fold tf join_abs acc0 (predecessor_list g v))"
+
+definition env_map :: "(pp => 'a abs_state) => (pp, 'a abs_state) map" where
+  "env_map env = (\<lambda>x. Some (env x))"
+
+definition lookup_bot :: "('x, 'd::bot) map => 'x => 'd" where
+  "lookup_bot m x = (case m x of None => bot | Some d => d)"
+
+lemma lookup_bot_env_map[simp]:
+  "lookup_bot (env_map env) x = env x"
+  unfolding lookup_bot_def env_map_def
+  by simp
+
+lemma mlup_env_map[simp]:
+  fixes env :: "pp \<Rightarrow> ('a::{bot}) abs_state"
+  shows "mlup (env_map env) x = env x"
+  unfolding mlup_def env_map_def by simp
+
+lemma rhs_tree_fold_traverse_env_map:
+  fixes env :: "pp \<Rightarrow> ('a::bounded_semilattice_sup_bot) abs_state"
+  shows "traverse_rhs (rhs_tree_fold tf join_abs acc ps) (env_map env)
+     = fold (\<lambda>(u,a) st. join_abs st (apply_tf tf a (env u))) ps acc"
+proof (induct ps arbitrary: acc)
+  case Nil
+  show ?case
+    by simp
+next
+  case (Cons p ps)
+  obtain u a where p: "p = (u, a)"
+    by (cases p) auto
+  have "traverse_rhs (rhs_tree_fold tf join_abs acc (p # ps)) (env_map env) =
+        traverse_rhs (Query u (\<lambda>su. rhs_tree_fold tf join_abs (join_abs acc (apply_tf tf a su)) ps))
+         (env_map env)"
+    by (simp add: p)
+  also have "\<dots> =
+        traverse_rhs (rhs_tree_fold tf join_abs (join_abs acc (apply_tf tf a (env u))) ps)
+         (env_map env)"
+    by simp
+  also have "\<dots> =
+        fold (\<lambda>(u,a) st. join_abs st (apply_tf tf a (env u))) ps
+         (join_abs acc (apply_tf tf a (env u)))"
+    using Cons[of "join_abs acc (apply_tf tf a (env u))"] by simp
+  also have "\<dots> =
+        fold (\<lambda>(u,a) st. join_abs st (apply_tf tf a (env u))) (p # ps) acc"
+    by (simp add: p)
+  finally show ?case .
+qed
+
+(* Avoid simp turning @{text "set xs = {}"} inside @{text SOME} into @{text "xs = []"} the wrong way. *)
+lemma SOME_list_distinct_set_empty_eq_Nil:
+  "(SOME xs :: ('a::type) list. distinct xs \<and> set xs = {}) = []"
+proof (rule some_equality)
+  show "distinct ([] :: 'a list) \<and> set [] = {}"
+    by simp
+next
+  fix xs :: "'a list"
+  assume H: "distinct xs \<and> set xs = {}"
+  then show "xs = []"
+    by simp
+qed
+
+lemma SOME_distinct_list_if_set_empty:
+  fixes P :: "'a set"
+  assumes hp: "P = {}"
+  shows "(SOME xs :: 'a list. distinct xs \<and> set xs = P) = []"
+  unfolding hp by (rule SOME_list_distinct_set_empty_eq_Nil)
+
+(* Special case: no edges into v and v is not the entry tree is Answer bot, same as rhs. *)
+lemma make_rhs_tree_eq_Answer_bot_if_no_preds_not_entry:
+  assumes not_e: "v \<noteq> cfg_entry g"
+  assumes no_in: "\<And>u a. (u, a, v) \<notin> edges g"
+  shows "make_rhs_tree g tf join_abs bot_abs s0 v = Answer bot_abs"
+  unfolding make_rhs_tree_def Let_def
+  using no_in not_e predecessor_list_Nil_if_no_in
+  by simp
+
+lemma make_rhs_tree_correspondence_not_entry_no_predecessors:
+  fixes env :: "pp \<Rightarrow> ('a::bounded_semilattice_sup_bot) abs_state"
+  assumes not_e: "v \<noteq> cfg_entry g"
+  assumes no_in: "\<And>u a. (u, a, v) \<notin> edges g"
+  shows "traverse_rhs (make_rhs_tree g tf join_abs bot_abs s0 v) (env_map env) =
+         make_rhs g tf join_abs bot_abs s0 v env"
+proof -
+  have tr: "traverse_rhs (make_rhs_tree g tf join_abs bot_abs s0 v) (env_map env) = bot_abs"
+    unfolding make_rhs_tree_eq_Answer_bot_if_no_preds_not_entry[OF not_e no_in] by simp
+  have mk: "make_rhs g tf join_abs bot_abs s0 v env = bot_abs"
+    unfolding make_rhs_def by (simp add: rhs_no_predecessors_not_entry not_e no_in)
+  from tr mk show ?thesis
+    by simp
+qed
+
+lemma finite_predecessor_pairs:
+  assumes fin: "finite (edges g)"
+  shows "finite {(u,a). (u,a,v) \<in> edges g}"
+proof (rule finite_subset)
+  show "{(u,a). (u,a,v) \<in> edges g} \<subseteq> (\<lambda>(u, a, w). (u, a)) ` edges g"
+    by force
+  show "finite ((\<lambda>(u, a, w). (u, a)) ` edges g)"
+    by (simp add: fin)
+qed
+
+lemma fold_join_apply_edges_eq_fold_join_over_map:
+  fixes join :: "'a \<Rightarrow> 'a \<Rightarrow> 'a" and F :: "('b \<times> 'c) \<Rightarrow> 'a"
+  shows "fold (\<lambda>p acc. join (F p) acc) ps acc =
+         fold (\<lambda>x acc. join x acc) (map F ps) acc"
+proof (induct ps arbitrary: acc)
+  case Nil
+  show ?case
+    by simp
+next
+  case (Cons p ps)
+  have "fold (\<lambda>p acc. join (F p) acc) (p # ps) acc =
+        fold (\<lambda>p acc. join (F p) acc) ps (join (F p) acc)"
+    by simp
+  also have "\<dots> = fold (\<lambda>x acc. join x acc) (map F ps) (join (F p) acc)"
+    using Cons[of "join (F p) acc"] by simp
+  also have "\<dots> = fold (\<lambda>x acc. join x acc) (map F (p # ps)) acc"
+    by simp
+  finally show ?case .
+qed
+
+lemma rhs_eq_fold_predecessors:
+  fixes g v tf join_abs bot_abs s0
+  fixes env :: "pp \<Rightarrow> ('a::bounded_semilattice_sup_bot) abs_state"
+  assumes fin: "finite (edges g)"
+  assumes cfi: "comp_fun_idem (join_abs :: 'a abs_state \<Rightarrow> 'a abs_state \<Rightarrow> 'a abs_state)"
+  assumes join_sym: "\<And>x y. join_abs x y = join_abs y x"
+  assumes dist: "distinct ps"
+  assumes setps: "set ps = {(u,a). (u,a,v) \<in> edges g}"
+  defines "preds \<equiv> {(u,a). (u,a,v) \<in> edges g}"
+  defines "F \<equiv> (\<lambda>(u,a). apply_tf tf a (env u))"
+  defines "vals \<equiv> F ` preds"
+  defines "acc0 \<equiv> (if v = cfg_entry g then join_abs bot_abs s0 else bot_abs)"
+  shows "rhs g tf join_abs bot_abs s0 env v =
+         fold (\<lambda>(u,a) acc. join_abs (apply_tf tf a (env u)) acc) ps acc0"
+proof -
+  interpret j: comp_fun_idem join_abs
+    by (fact cfi)
+  have fin_preds: "finite preds"
+    unfolding preds_def by (rule finite_predecessor_pairs[OF fin])
+  have setps': "set ps = preds"
+    unfolding preds_def using setps by simp
+  have vals_eq: "vals = set (map F ps)"
+    unfolding vals_def using setps' by simp
+  have fold_map:
+    "fold (\<lambda>(u,a) acc. join_abs (apply_tf tf a (env u)) acc) ps acc0 =
+     fold (\<lambda>x acc. join_abs x acc) (map F ps) acc0"
+  proof -
+    have H: "(\<lambda>(u,a) acc. join_abs (apply_tf tf a (env u)) acc) = (\<lambda>p acc. join_abs (F p) acc)"
+      by (rule ext)+ (simp add: F_def split: prod.split)
+    show ?thesis
+      unfolding H by (rule fold_join_apply_edges_eq_fold_join_over_map)
+  qed
+  have fold_set:
+    "Finite_Set.fold join_abs acc0 (set (map F ps)) =
+     fold (\<lambda>x acc. join_abs x acc) (map F ps) acc0"
+    by (rule j.fold_set_fold)
+  show ?thesis
+  proof (cases "v = cfg_entry g")
+    case True
+    have rhsv: "rhs g tf join_abs bot_abs s0 env v = abs_join_set join_abs bot_abs (insert s0 vals)"
+      unfolding rhs_def preds_def vals_def F_def using True by (simp add: Let_def)
+    have fin_vals: "finite vals"
+      unfolding vals_def using fin_preds by simp
+    have ins_fold:
+      "Finite_Set.fold join_abs bot_abs (insert s0 vals) =
+       Finite_Set.fold join_abs (join_abs s0 bot_abs) vals"
+      by (simp only: j.fold_insert_idem2 fin_vals)
+    also have "join_abs s0 bot_abs = join_abs bot_abs s0"
+      by (simp add: join_sym)
+    also have "Finite_Set.fold join_abs (join_abs bot_abs s0) vals =
+               Finite_Set.fold join_abs acc0 (set (map F ps))"
+      unfolding vals_eq acc0_def using True by simp
+    also have "\<dots> = fold (\<lambda>x acc. join_abs x acc) (map F ps) acc0"
+      by (simp add: fold_set[symmetric])
+    also have "\<dots> = fold (\<lambda>(u,a) acc. join_abs (apply_tf tf a (env u)) acc) ps acc0"
+      by (simp add: fold_map[symmetric])
+    finally show ?thesis
+      unfolding rhsv abs_join_set_def by simp
+  next
+    case False
+    then have ne: "v \<noteq> cfg_entry g"
+      by simp
+    have rhsv: "rhs g tf join_abs bot_abs s0 env v = abs_join_set join_abs bot_abs vals"
+      unfolding rhs_def preds_def vals_def F_def using False by (simp add: Let_def)
+    have "Finite_Set.fold join_abs bot_abs vals =
+          Finite_Set.fold join_abs acc0 (set (map F ps))"
+      unfolding vals_eq acc0_def using ne by simp
+    also have "\<dots> = fold (\<lambda>x acc. join_abs x acc) (map F ps) acc0"
+      by (simp add: fold_set[symmetric])
+    also have "\<dots> = fold (\<lambda>(u,a) acc. join_abs (apply_tf tf a (env u)) acc) ps acc0"
+      by (simp add: fold_map[symmetric])
+    finally show ?thesis
+      unfolding rhsv abs_join_set_def by simp
+  qed
+qed
+
+lemma rhs_eq_fold_predecessor_list:
+  fixes g v tf join_abs bot_abs s0
+  fixes env :: "pp \<Rightarrow> ('a::bounded_semilattice_sup_bot) abs_state"
+  assumes fin: "finite (edges g)"
+  assumes cfi: "comp_fun_idem (join_abs :: 'a abs_state \<Rightarrow> 'a abs_state \<Rightarrow> 'a abs_state)"
+  assumes join_sym: "\<And>x y. join_abs x y = join_abs y x"
+  shows "rhs g tf join_abs bot_abs s0 env v =
+         fold (\<lambda>(u,a) acc. join_abs (apply_tf tf a (env u)) acc)
+              (predecessor_list g v)
+              (if v = cfg_entry g then join_abs bot_abs s0 else bot_abs)"
+proof -
+  have setps: "set (predecessor_list g v) = {(u,a). (u,a,v) \<in> edges g}"
+    using set_predecessor_list[OF fin] unfolding predecessors_def by auto
+  show ?thesis
+    using rhs_eq_fold_predecessors[OF fin cfi join_sym
+        distinct_predecessor_list[OF fin] setps]
+    by simp
+qed
+
+lemma fold_join_abs_swap_edge_steps:
+  fixes join_abs :: "'a::bounded_semilattice_sup_bot abs_state \<Rightarrow> 'a abs_state \<Rightarrow> 'a abs_state"
+    and tf :: "'a domain_transfer"
+    and env :: "pp \<Rightarrow> 'a abs_state"
+  assumes join_sym: "\<And>x y. join_abs x y = join_abs y x"
+  shows "fold (\<lambda>(u,a) st. join_abs st (apply_tf tf a (env u))) ps acc =
+         fold (\<lambda>(u,a) acc. join_abs (apply_tf tf a (env u)) acc) ps acc"
+proof (induct ps arbitrary: acc)
+  case Nil
+  show ?case
+    by simp
+next
+  case (Cons p ps)
+  obtain u a where pa: "p = (u, a)"
+    by (cases p) auto
+  have "fold (\<lambda>(u,a) st. join_abs st (apply_tf tf a (env u))) (p # ps) acc =
+        fold (\<lambda>(u,a) st. join_abs st (apply_tf tf a (env u))) ps (join_abs acc (apply_tf tf a (env u)))"
+    by (simp add: pa)
+  also have "join_abs acc (apply_tf tf a (env u)) = join_abs (apply_tf tf a (env u)) acc"
+    by (simp add: join_sym)
+  also have "fold (\<lambda>(u,a) st. join_abs st (apply_tf tf a (env u))) ps (join_abs (apply_tf tf a (env u)) acc) =
+             fold (\<lambda>(u,a) acc. join_abs (apply_tf tf a (env u)) acc) ps (join_abs (apply_tf tf a (env u)) acc)"
+    using Cons.hyps by simp
+  also have "\<dots> = fold (\<lambda>(u,a) acc. join_abs (apply_tf tf a (env u)) acc) (p # ps) acc"
+    by (simp add: pa)
+  finally show ?case .
+qed
+
+lemma make_rhs_tree_correspondence:
+  assumes fin: "finite (edges g)"
+  assumes cfi: "comp_fun_idem (join_abs :: 'a::bounded_semilattice_sup_bot abs_state \<Rightarrow> 'a abs_state \<Rightarrow> 'a abs_state)"
+  assumes join_sym: "\<And>x y. join_abs x y = join_abs y x"
+  shows "traverse_rhs (make_rhs_tree g tf join_abs bot_abs s0 v) (env_map (env :: pp \<Rightarrow> 'a abs_state)) =
+         make_rhs g tf join_abs bot_abs s0 v env"
+proof -
+  have "traverse_rhs (make_rhs_tree g tf join_abs bot_abs s0 v) (env_map env) =
+        fold (\<lambda>(u,a) st. join_abs st (apply_tf tf a (env u)))
+             (predecessor_list g v)
+             (if v = cfg_entry g then join_abs bot_abs s0 else bot_abs)"
+    unfolding make_rhs_tree_def Let_def
+    by (simp add: rhs_tree_fold_traverse_env_map)
+  also have "\<dots> =
+        fold (\<lambda>(u,a) acc. join_abs (apply_tf tf a (env u)) acc)
+             (predecessor_list g v)
+             (if v = cfg_entry g then join_abs bot_abs s0 else bot_abs)"
+    by (rule fold_join_abs_swap_edge_steps[OF join_sym])
+  also have "\<dots> = rhs g tf join_abs bot_abs s0 env v"
+    by (simp add: rhs_eq_fold_predecessor_list[OF fin cfi join_sym])
+  finally show ?thesis
+    unfolding make_rhs_def by (simp split: if_splits)
+qed
+
+lemma mlup_env_map_of_mlup:
+  fixes \<sigma> :: "(pp, ('a::bounded_semilattice_sup_bot) abs_state) map"
+  shows "mlup (env_map (\<lambda>w. mlup \<sigma> w)) x = mlup \<sigma> x"
+  by (simp add: mlup_env_map)
+
+lemma lookup_bot_mlup:
+  fixes \<sigma> :: "(pp, ('a::bounded_semilattice_sup_bot) abs_state) map"
+  shows "lookup_bot \<sigma> x = mlup \<sigma> x"
+  unfolding lookup_bot_def mlup_def by (cases "\<sigma> x") simp_all
+
+lemma traverse_rhs_mlup_eq:
+  fixes t :: "(pp, ('a::bounded_semilattice_sup_bot) abs_state) strategy_tree"
+    and \<sigma> \<sigma>' :: "(pp, ('a::bounded_semilattice_sup_bot) abs_state) map"
+  assumes mlup_ag: "\<And>z. mlup \<sigma> z = mlup \<sigma>' z"
+  shows "traverse_rhs t \<sigma> = traverse_rhs t \<sigma>'"
+  apply (rule solution_sufficient_t)
+  using mlup_ag by simp
+
+lemma rhs_make_rhs_tree_traverse_mlup:
+  fixes g :: cfg and tf :: "'a::bounded_semilattice_sup_bot domain_transfer"
+    and join_abs bot_abs s0 v and \<sigma> :: "(pp, ('a::bounded_semilattice_sup_bot) abs_state) map"
+  assumes fin: "finite (edges g)"
+  assumes cfi: "comp_fun_idem (join_abs :: 'a abs_state \<Rightarrow> 'a abs_state \<Rightarrow> 'a abs_state)"
+  assumes join_sym: "\<And>x y. join_abs x y = join_abs y x"
+  shows "rhs g tf join_abs bot_abs s0 (\<lambda>w. mlup \<sigma> w) v =
+         traverse_rhs (make_rhs_tree g tf join_abs bot_abs s0 v) \<sigma>"
+proof -
+  have "traverse_rhs (make_rhs_tree g tf join_abs bot_abs s0 v) \<sigma> =
+        traverse_rhs (make_rhs_tree g tf join_abs bot_abs s0 v) (env_map (\<lambda>w. mlup \<sigma> w))"
+    by (rule traverse_rhs_mlup_eq) (simp add: mlup_env_map_of_mlup)
+  also have "\<dots> =
+        make_rhs g tf join_abs bot_abs s0 v (\<lambda>w. mlup \<sigma> w)"
+    by (simp add: make_rhs_tree_correspondence[OF fin cfi join_sym])
+  also have "\<dots> = rhs g tf join_abs bot_abs s0 (\<lambda>w. mlup \<sigma> w) v"
+    by (simp add: make_rhs_def)
+  finally show ?thesis ..
+qed
+
+(* -- CFG + strategy forest (shared by all TD backends) -- *)
+
+lemma eq_le_mlup_imp_rhs_le:
+  fixes g :: cfg and tf :: "'a::bounded_semilattice_sup_bot domain_transfer"
+    and join_abs :: "'a abs_state \<Rightarrow> 'a abs_state \<Rightarrow> 'a abs_state"
+    and bot_abs s0 :: "'a abs_state"
+    and T :: "pp \<Rightarrow> (pp, 'a abs_state) strategy_tree"
+    and \<sigma> :: "(pp, 'a abs_state) map" and v :: pp
+  assumes T_mk: "\<And>w. T w = make_rhs_tree g tf join_abs bot_abs s0 w"
+  assumes fin: "finite (edges g)"
+  assumes cfi: "comp_fun_idem join_abs"
+  assumes join_sym: "\<And>x y. join_abs x y = join_abs y x"
+  assumes le: "(eq T) v \<sigma> \<le> mlup \<sigma> v"
+  shows "rhs g tf join_abs bot_abs s0 (\<lambda>w. lookup_bot \<sigma> w) v \<le> lookup_bot \<sigma> v"
+proof -
+  have "rhs g tf join_abs bot_abs s0 (\<lambda>w. lookup_bot \<sigma> w) v =
+        rhs g tf join_abs bot_abs s0 (\<lambda>w. mlup \<sigma> w) v"
+    by (simp add: fun_eq_iff lookup_bot_mlup)
+  also have "\<dots> = traverse_rhs (T v) \<sigma>"
+  proof -
+    have "rhs g tf join_abs bot_abs s0 (\<lambda>w. mlup \<sigma> w) v =
+          traverse_rhs (make_rhs_tree g tf join_abs bot_abs s0 v) \<sigma>"
+      by (rule rhs_make_rhs_tree_traverse_mlup[OF fin cfi join_sym])
+    thus ?thesis unfolding T_mk by simp
+  qed
+  also have "traverse_rhs (T v) \<sigma> = (eq T) v \<sigma>"
+    by (simp add: eq_def)
+  also have "\<dots> \<le> mlup \<sigma> v"
+    using le by simp
+  finally show ?thesis
+    by (simp add: lookup_bot_mlup)
+qed
+
+lemma cfg_env_post_fixpoint:
+  fixes g :: cfg and tf :: "'a::bounded_semilattice_sup_bot domain_transfer"
+    and join_abs :: "'a abs_state \<Rightarrow> 'a abs_state \<Rightarrow> 'a abs_state"
+    and bot_abs s0 :: "'a abs_state"
+    and T :: "pp \<Rightarrow> (pp, 'a abs_state) strategy_tree"
+    and env :: "pp \<Rightarrow> 'a abs_state" and \<sigma> :: "(pp, 'a abs_state) map"
+  assumes T_mk: "\<And>w. T w = make_rhs_tree g tf join_abs bot_abs s0 w"
+  assumes fin: "finite (edges g)"
+  assumes cfi: "comp_fun_idem join_abs"
+  assumes join_sym: "\<And>x y. join_abs x y = join_abs y x"
+  assumes env_def: "\<And>w. env w = lookup_bot \<sigma> w"
+  assumes eq_le: "\<And>v. (eq T) v \<sigma> \<le> mlup \<sigma> v"
+  shows "is_post_fixpoint g tf join_abs bot_abs s0 env"
+  unfolding is_post_fixpoint_def
+proof (intro allI)
+  fix v
+  show "rhs g tf join_abs bot_abs s0 env v \<le> env v"
+  proof -
+    have "rhs g tf join_abs bot_abs s0 env v \<le> lookup_bot \<sigma> v"
+      using eq_le_mlup_imp_rhs_le[OF T_mk fin cfi join_sym eq_le] env_def by presburger
+    thus ?thesis using env_def by simp
+  qed
+qed
+
+locale td_cfg_core =
+  fixes g :: cfg and
+  tf :: "'a::bounded_semilattice_sup_bot domain_transfer" and
+  join_abs :: "'a abs_state \<Rightarrow> 'a abs_state \<Rightarrow> 'a abs_state" and
+  bot_abs s0 :: "'a abs_state"
+begin
+
+definition cfg_T :: "pp \<Rightarrow> (pp, 'a abs_state) strategy_tree"
+where
+  "cfg_T v = make_rhs_tree g tf join_abs bot_abs s0 v"
+
+lemma cfg_T_eq[simp]:
+  "cfg_T v = make_rhs_tree g tf join_abs bot_abs s0 v"
+  unfolding cfg_T_def by rule
+
+lemma cfg_env_post_fixpoint:
+  fixes env :: "pp \<Rightarrow> 'a abs_state" and \<sigma> :: "(pp, 'a abs_state) map"
+  assumes fin: "finite (edges g)"
+  assumes cfi: "comp_fun_idem join_abs"
+  assumes join_sym: "\<And>x y. join_abs x y = join_abs y x"
+  assumes env_def: "\<And>w. env w = lookup_bot \<sigma> w"
+  assumes eq_le: "\<And>v. (eq cfg_T) v \<sigma> \<le> mlup \<sigma> v"
+  shows "is_post_fixpoint g tf join_abs bot_abs s0 env"
+  using cfg_env_post_fixpoint[where T=cfg_T, OF cfg_T_eq fin cfi join_sym env_def eq_le]
+  by simp
+
+end
+
+end
