src/Solver/TD_WN_Interface.thy
@@ -1,0 +1,136 @@
+theory TD_WN_Interface
+  imports TD_CFG_Core "TD.TD_wn_post"
+begin
+
+(*
+  Full W/N backend (TD_wn_post): widening and narrowing phases, destabilization.
+  Uses TD_CFG_Core for make_rhs_tree and is_post_fixpoint readback.
+*)
+
+definition widen_abs ::
+    "('a::bounded_lattice \<Rightarrow> 'a \<Rightarrow> 'a)
+     \<Rightarrow> 'a abs_state
+     \<Rightarrow> 'a abs_state
+     \<Rightarrow> 'a abs_state"
+where
+  "widen_abs widen s1 s2 x = widen (s1 x) (s2 x)"
+
+definition narrow_abs ::
+    "('a::bounded_lattice \<Rightarrow> 'a \<Rightarrow> 'a)
+     \<Rightarrow> 'a abs_state
+     \<Rightarrow> 'a abs_state
+     \<Rightarrow> 'a abs_state"
+where
+  "narrow_abs narrow s1 s2 x = narrow (s1 x) (s2 x)"
+
+lemma widen_abs_ge:
+  fixes widen :: "'a::bounded_lattice \<Rightarrow> 'a \<Rightarrow> 'a"
+  assumes "\<And>a b. a \<squnion> b \<le> widen a b"
+  shows "s1 \<squnion> s2 \<le> widen_abs widen s1 s2"
+  unfolding widen_abs_def le_fun_def
+proof (intro allI)
+  fix x
+  show "(s1 \<squnion> s2) x \<le> widen (s1 x) (s2 x)"
+    using assms[of "s1 x" "s2 x"] by simp
+qed
+
+lemma narrow_abs_ge:
+  fixes narrow :: "'a::bounded_lattice \<Rightarrow> 'a \<Rightarrow> 'a"
+  assumes "\<And>a b. a \<sqinter> b \<le> narrow a b"
+  shows "s1 \<sqinter> s2 \<le> narrow_abs narrow s1 s2"
+  unfolding narrow_abs_def le_fun_def
+proof (intro allI)
+  fix x
+  show "(s1 \<sqinter> s2) x \<le> narrow (s1 x) (s2 x)"
+    using assms[of "s1 x" "s2 x"] by simp
+qed
+
+lemma narrow_abs_le:
+  fixes narrow :: "'a::bounded_lattice \<Rightarrow> 'a \<Rightarrow> 'a"
+  assumes "\<And>a b. narrow a b \<le> a"
+  shows "narrow_abs narrow s1 s2 \<le> s1"
+  unfolding narrow_abs_def le_fun_def by (simp add: assms)
+
+lemma reach_in_stabl:
+  fixes T :: "pp \<Rightarrow> (pp, 'd::order_bot) strategy_tree" and x :: pp and stabl :: "pp set"
+    and sigma :: "(pp, 'd) map"
+  assumes post: "part_post_solution T x sigma stabl"
+  assumes x_in: "x \<in> stabl"
+  assumes v_reach: "v \<in> reach T sigma x"
+  shows "v \<in> stabl"
+  using v_reach proof induct
+  case base
+  then show ?case using x_in by simp
+next
+  case (step y z)
+  then have y_stabl: "y \<in> stabl" by simp
+  then have "dep T sigma y \<subseteq> stabl"
+    by (simp add: post)
+  then show ?case using step.hyps(3) by auto
+qed
+
+locale td_cfg_wn_solver =
+  fixes g :: cfg and
+  tf :: "'a::bounded_lattice domain_transfer" and
+  join_abs :: "'a abs_state \<Rightarrow> 'a abs_state \<Rightarrow> 'a abs_state" and
+  bot_abs s0 :: "'a abs_state" and
+  widen narrow :: "'a abs_state \<Rightarrow> 'a abs_state \<Rightarrow> 'a abs_state"
+  assumes widen_ge: "s1 \<squnion> s2 \<le> widen s1 s2"
+  assumes widen_bounded: "s2 \<le> s1 \<Longrightarrow> widen s1 s2 = s1"
+  assumes narrow_ge: "s1 \<sqinter> s2 \<le> narrow s1 s2"
+  assumes narrow_le: "narrow s1 s2 \<le> s1"
+begin
+
+definition cfg_T :: "pp \<Rightarrow> (pp, 'a abs_state) strategy_tree"
+where
+  "cfg_T v = make_rhs_tree g tf join_abs bot_abs s0 v"
+
+interpretation td_wn: TD_wn_post cfg_T widen narrow
+  using TD_wn_post.intro narrow_ge narrow_le widen_bounded widen_ge by blast
+
+definition td_wn_sigma :: "(pp, 'a abs_state) map"
+where
+  "td_wn_sigma = snd (td_wn.solve (cfg_entry g))"
+
+definition td_wn_env :: "pp \<Rightarrow> 'a abs_state"
+where
+  "td_wn_env v = lookup_bot td_wn_sigma v"
+
+lemma td_wn_eq_le_on_reach:
+  fixes stabl :: "pp set" and sigma :: "(pp, 'a abs_state) map"
+  assumes mono: "is_mono_eq cfg_T"
+  assumes deps: "mono_deps cfg_T"
+  assumes dom: "td_wn.solve_dom (cfg_entry g)"
+  assumes sol: "td_wn.solve (cfg_entry g) = (stabl, sigma)"
+  assumes v_reach: "v \<in> reach cfg_T sigma (cfg_entry g)"
+  shows "(eq cfg_T) v sigma \<le> mlup sigma v"
+proof -
+  have post: "part_post_solution cfg_T (cfg_entry g) sigma stabl"
+    using td_wn.partial_correctness[OF mono deps dom sol] by simp
+  then have entry_stabl: "cfg_entry g \<in> stabl" by blast
+  have v_stabl: "v \<in> stabl"
+    using post reach_in_stabl v_reach entry_stabl by blast
+  show ?thesis using post v_stabl by fastforce
+qed
+
+lemma td_wn_env_post_fixpoint:
+  assumes fin: "finite (edges g)"
+  assumes cfi: "comp_fun_idem join_abs"
+  assumes join_sym: "\<And>x y. join_abs x y = join_abs y x"
+  assumes mono: "is_mono_eq cfg_T"
+  assumes deps: "mono_deps cfg_T"
+  assumes dom: "td_wn.solve_dom (cfg_entry g)"
+  assumes reach: "\<And>v. v \<in> reach cfg_T td_wn_sigma (cfg_entry g)"
+  shows "is_post_fixpoint g tf join_abs bot_abs s0 td_wn_env"
+proof -
+  obtain stabl sigma where sol: "td_wn.solve (cfg_entry g) = (stabl, sigma)"
+    and sigma_eq: "td_wn_sigma = sigma"
+    unfolding td_wn_sigma_def by (metis prod.collapse)
+  show ?thesis
+    using cfg_env_post_fixpoint[where T=cfg_T, OF cfg_T_def fin cfi join_sym]
+    using deps dom mono reach sigma_eq sol td_wn_env_def td_wn_eq_le_on_reach by blast
+qed
+
+end
+
+end
